lib/monads/trace: update definitions and rules taken from nondet
This commit has all of the changes required so that the definitions and
rules added in the previous commit work for the trace monad.

Signed-off-by: Corey Lewis <corey.lewis@proofcraft.systems>

lib/Monads/trace/Trace_Monad.thy
@@ -47,21 +47,22 @@ text \<open>
 type_synonym ('s, 'a) tmonad = "'s \<Rightarrow> ((tmid \<times> 's) list \<times> ('s, 'a) tmres) set"
 
 text \<open>
-  Print the type @{typ "('s,'a) nondet_monad"} instead of its unwieldy expansion.
+  Print the type @{typ "('s,'a) tmonad"} instead of its unwieldy expansion.
   Needs an AST translation in code, because it needs to check that the state variable
-  @{typ 's} occurs twice. This comparison is not guaranteed to always work as expected
+  @{typ 's} occurs three times. This comparison is not guaranteed to always work as expected
   (AST instances might have different decoration), but it does seem to work here.\<close>
 print_ast_translation \<open>
   let
-    fun monad_tr _ [t1, Ast.Appl [Ast.Constant @{type_syntax prod},
-                          Ast.Appl [Ast.Constant @{type_syntax set},
-                            Ast.Appl [Ast.Constant @{type_syntax prod}, t2, t3]],
-                          Ast.Constant @{type_syntax bool}]] =
-      if t3 = t1
-      then Ast.Appl [Ast.Constant @{type_syntax "nondet_monad"}, t1, t2]
+    fun tmonad_tr _ [t1, Ast.Appl [Ast.Constant @{type_syntax set},
+                          Ast.Appl [Ast.Constant @{type_syntax prod},
+                            Ast.Appl [Ast.Constant @{type_syntax list},
+                              Ast.Appl [Ast.Constant @{type_syntax prod},
+                                Ast.Constant @{type_syntax tmid}, t2]],
+                            Ast.Appl [Ast.Constant @{type_syntax tmres}, t3, t4]]]] =
+      if t1 = t2 andalso t1 = t3
+      then Ast.Appl [Ast.Constant @{type_syntax "tmonad"}, t1, t4]
       else raise Match
-  in [(@{type_syntax "fun"}, monad_tr)] end
-\<close>
+  in [(@{type_syntax "fun"}, tmonad_tr)] end\<close>
 
 text \<open>Returns monad results, ignoring failures and traces.\<close>
 definition mres :: "((tmid \<times> 's) list \<times> ('s, 'a) tmres) set \<Rightarrow> ('a \<times> 's) set" where
@@ -141,11 +142,16 @@ text \<open>
   FIXME: The @{text select_f} function was left out here until we figure
   out what variant we actually need.\<close>
 
-text \<open>@{text select_state} takes a relationship between
-  states, and outputs nondeterministically a state
-  related to the input state.\<close>
-definition state_select :: "('s \<times> 's) set \<Rightarrow> ('s, unit) nondet_monad" where
-  "state_select r \<equiv> \<lambda>s. ((\<lambda>x. ((), x)) ` {s'. (s, s') \<in> r}, \<not> (\<exists>s'. (s, s') \<in> r))"
+definition
+  "default_elem dflt A \<equiv> if A = {} then {dflt} else A"
+
+text \<open>
+  @{text state_select} takes a relationship between states, and outputs
+  nondeterministically a state related to the input state. Fails if no such
+  state exists.\<close>
+definition state_select :: "('s \<times> 's) set \<Rightarrow> ('s, unit) tmonad" where
+  "state_select r \<equiv>
+     \<lambda>s. (Pair [] ` default_elem Failed (Result ` (\<lambda>x. ((), x)) ` {s'. (s, s') \<in> r}))"
 
 subsection "Failure"
 
@@ -212,7 +218,7 @@ text \<open>
   Get a map (such as a heap) from the current state and apply an argument to the map.
   Fail if the map returns @{const None}, otherwise return the value.\<close>
 definition
-  gets_map :: "('s \<Rightarrow> 'a \<Rightarrow> 'b option) \<Rightarrow> 'a \<Rightarrow> ('s, 'b) nondet_monad" where
+  gets_map :: "('s \<Rightarrow> 'a \<Rightarrow> 'b option) \<Rightarrow> 'a \<Rightarrow> ('s, 'b) tmonad" where
   "gets_map f p \<equiv> gets f >>= (\<lambda>m. assert_opt (m p))"
 
 
@@ -520,8 +526,8 @@ text \<open>The same for the exception monad:\<close>
 definition liftME :: "('a \<Rightarrow> 'b) \<Rightarrow> ('s,'e+'a) tmonad \<Rightarrow> ('s,'e+'b) tmonad" where
   "liftME f m \<equiv> doE x \<leftarrow> m; returnOk (f x) odE"
 
-text \<open> Execute @{term f} for @{term "Some x"}, otherwise do nothing. \<close>
-definition maybeM :: "('a \<Rightarrow> ('s, unit) nondet_monad) \<Rightarrow> 'a option \<Rightarrow> ('s, unit) nondet_monad" where
+text \<open>Execute @{term f} for @{term "Some x"}, otherwise do nothing.\<close>
+definition maybeM :: "('a \<Rightarrow> ('s, unit) tmonad) \<Rightarrow> 'a option \<Rightarrow> ('s, unit) tmonad" where
   "maybeM f y \<equiv> case y of Some x \<Rightarrow> f x | None \<Rightarrow> return ()"
 
 text \<open>Run a sequence of monads from left to right, ignoring return values.\<close>
@@ -589,10 +595,8 @@ primrec filterM :: "('a \<Rightarrow> ('s, bool) tmonad) \<Rightarrow> 'a list \
      return (if b then (x # ys) else ys)
    od"
 
-text \<open>
-  @{text select_state} takes a relationship between states, and outputs
-  nondeterministically a state related to the input state.\<close>
-definition state_select :: "('s \<times> 's) set \<Rightarrow> ('s, unit) tmonad" where
+text \<open>An alternative definition of @{term state_select}\<close>
+lemma state_select_def2:
   "state_select r \<equiv> (do
     s \<leftarrow> get;
     S \<leftarrow> return {s'. (s, s') \<in> r};
@@ -600,6 +604,11 @@ definition state_select :: "('s \<times> 's) set \<Rightarrow> ('s, unit) tmonad
     s' \<leftarrow> select S;
     put s'
   od)"
+  apply (clarsimp simp add: state_select_def get_def return_def assert_def fail_def select_def
+                            put_def bind_def fun_eq_iff default_elem_def
+                    intro!: eq_reflection)
+  apply fastforce
+  done
 
 
 section "Catching and Handling Exceptions"
@@ -715,44 +724,45 @@ notation (output)
 
 section "Combinators that have conditions with side effects"
 
-definition notM :: "('s, bool) nondet_monad \<Rightarrow> ('s, bool) nondet_monad" where
+definition notM :: "('s, bool) tmonad \<Rightarrow> ('s, bool) tmonad" where
   "notM m = do c \<leftarrow> m; return (\<not> c) od"
 
-definition
-  whileM :: "('s, bool) nondet_monad \<Rightarrow> ('s, 'a) nondet_monad \<Rightarrow> ('s, unit) nondet_monad" where
+definition whileM ::
+  "('s, bool) tmonad \<Rightarrow> ('s, 'a) tmonad \<Rightarrow> ('s, unit) tmonad" where
   "whileM C B \<equiv> do
     c \<leftarrow> C;
     whileLoop (\<lambda>c s. c) (\<lambda>_. do B; C od) c;
     return ()
   od"
 
-definition
-  ifM :: "('s, bool) nondet_monad \<Rightarrow> ('s, 'a) nondet_monad \<Rightarrow> ('s, 'a) nondet_monad \<Rightarrow>
-          ('s, 'a) nondet_monad" where
+definition ifM ::
+  "('s, bool) tmonad \<Rightarrow> ('s, 'a) tmonad \<Rightarrow> ('s, 'a) tmonad \<Rightarrow>
+          ('s, 'a) tmonad" where
   "ifM test t f = do
     c \<leftarrow> test;
     if c then t else f
    od"
 
 definition ifME ::
-  "('a, 'b + bool) nondet_monad \<Rightarrow> ('a, 'b + 'c) nondet_monad \<Rightarrow> ('a, 'b + 'c) nondet_monad
-   \<Rightarrow> ('a, 'b + 'c) nondet_monad" where
+  "('a, 'b + bool) tmonad \<Rightarrow> ('a, 'b + 'c) tmonad \<Rightarrow> ('a, 'b + 'c) tmonad
+   \<Rightarrow> ('a, 'b + 'c) tmonad" where
   "ifME test t f = doE
     c \<leftarrow> test;
     if c then t else f
    odE"
 
-definition
-  whenM :: "('s, bool) nondet_monad \<Rightarrow> ('s, unit) nondet_monad \<Rightarrow> ('s, unit) nondet_monad" where
+definition whenM ::
+  "('s, bool) tmonad \<Rightarrow> ('s, unit) tmonad \<Rightarrow> ('s, unit) tmonad" where
   "whenM t m = ifM t m (return ())"
 
-definition
-  orM :: "('s, bool) nondet_monad \<Rightarrow> ('s, bool) nondet_monad \<Rightarrow> ('s, bool) nondet_monad" where
+definition orM ::
+  "('s, bool) tmonad \<Rightarrow> ('s, bool) tmonad \<Rightarrow> ('s, bool) tmonad" where
   "orM a b = ifM a (return True) b"
 
 definition
-  andM :: "('s, bool) nondet_monad \<Rightarrow> ('s, bool) nondet_monad \<Rightarrow> ('s, bool) nondet_monad" where
+  andM :: "('s, bool) tmonad \<Rightarrow> ('s, bool) tmonad \<Rightarrow> ('s, bool) tmonad" where
   "andM a b = ifM a b (return False)"
+
 
 subsection "Await command"
 
