lib/Monads/trace/Trace_Monad_Equations.thy
@@ -29,11 +29,7 @@ lemma exec_modify:
 
 lemma bind_return_eq:
   "(a >>= return) = (b >>= return) \<Longrightarrow> a = b"
-  apply (clarsimp simp:bind_def)
-  apply (rule ext)
-  apply (drule_tac x= x in fun_cong)
-  apply (auto simp:return_def split_def)
-  done
+  by clarsimp
 
 lemmas bind_then_eq = arg_cong2[where f=bind, OF _ refl]
 
@@ -51,7 +47,7 @@ lemma throwError_bind:
 
 lemma bind_bindE_assoc:
   "((f >>= g) >>=E h)
-    = f >>= (\<lambda>rv. g rv >>=E h)"
+   = f >>= (\<lambda>rv. g rv >>=E h)"
   by (simp add: bindE_def bind_assoc)
 
 lemma returnOk_bind:
@@ -71,7 +67,7 @@ lemma cart_singleton_image:
 
 lemma liftE_bindE_handle:
   "((liftE f >>=E (\<lambda>x. g x)) <handle> h)
-      = f >>= (\<lambda>x. g x <handle> h)"
+   = f >>= (\<lambda>x. g x <handle> h)"
   by (simp add: liftE_bindE handleE_def handleE'_def
                 bind_assoc)
 
@@ -93,13 +89,13 @@ lemma liftE_bindE_assoc:
 
 lemma unlessE_throw_catch_If:
   "catch (unlessE P (throwError e) >>=E f) g
-      = (if P then catch (f ()) g else g e)"
+   = (if P then catch (f ()) g else g e)"
   by (simp add: unlessE_def catch_throwError split: if_split)
 
 lemma whenE_bindE_throwError_to_if:
   "whenE P (throwError e) >>=E (\<lambda>_. b) = (if P then (throwError e) else b)"
   unfolding whenE_def bindE_def
-  by (auto simp: Nondet_Monad.lift_def throwError_def returnOk_def)
+  by (auto simp: lift_def throwError_def returnOk_def)
 
 lemma alternative_liftE_returnOk:
   "(liftE m \<sqinter> returnOk v) = liftE (m \<sqinter> return v)"
@@ -129,13 +125,13 @@ lemma all_rv_choice_fn_eq_pred:
 
 lemma all_rv_choice_fn_eq:
   "\<lbrakk> \<And>rv. \<exists>fn. f rv = g fn \<rbrakk>
-    \<Longrightarrow> \<exists>fn. f = (\<lambda>rv. g (fn rv))"
+   \<Longrightarrow> \<exists>fn. f = (\<lambda>rv. g (fn rv))"
   using all_rv_choice_fn_eq_pred[where f=f and g=g and P=\<top>]
   by (simp add: fun_eq_iff)
 
 lemma gets_the_eq_bind:
   "\<lbrakk> \<exists>fn. f = gets_the (fn o fn'); \<And>rv. \<exists>fn. g rv = gets_the (fn o fn') \<rbrakk>
-     \<Longrightarrow> \<exists>fn. (f >>= g) = gets_the (fn o fn')"
+   \<Longrightarrow> \<exists>fn. (f >>= g) = gets_the (fn o fn')"
   apply (clarsimp dest!: all_rv_choice_fn_eq)
   apply (rule_tac x="\<lambda>s. case (fn s) of None \<Rightarrow> None | Some v \<Rightarrow> fna v s" in exI)
   apply (simp add: gets_the_def bind_assoc exec_gets
@@ -145,7 +141,7 @@ lemma gets_the_eq_bind:
 
 lemma gets_the_eq_bindE:
   "\<lbrakk> \<exists>fn. f = gets_the (fn o fn'); \<And>rv. \<exists>fn. g rv = gets_the (fn o fn') \<rbrakk>
-     \<Longrightarrow> \<exists>fn. (f >>=E g) = gets_the (fn o fn')"
+   \<Longrightarrow> \<exists>fn. (f >>=E g) = gets_the (fn o fn')"
   apply (simp add: bindE_def)
   apply (erule gets_the_eq_bind)
   apply (simp add: lift_def gets_the_returns split: sum.split)
@@ -171,9 +167,9 @@ lemma ex_const_function:
 
 lemma gets_the_condsE:
   "(\<exists>fn. whenE P f = gets_the (fn o fn'))
-            = (P \<longrightarrow> (\<exists>fn. f = gets_the (fn o fn')))"
+   = (P \<longrightarrow> (\<exists>fn. f = gets_the (fn o fn')))"
   "(\<exists>fn. unlessE P g = gets_the (fn o fn'))
-            = (\<not> P \<longrightarrow> (\<exists>fn. g = gets_the (fn o fn')))"
+   = (\<not> P \<longrightarrow> (\<exists>fn. g = gets_the (fn o fn')))"
   by (simp add: whenE_def unlessE_def gets_the_returns ex_const_function
          split: if_split)+
 
@@ -187,7 +183,7 @@ lemma liftME_return:
 
 lemma fold_bindE_into_list_case:
   "(doE v \<leftarrow> f; case_list (g v) (h v) x odE)
-      = (case_list (doE v \<leftarrow> f; g v odE) (\<lambda>x xs. doE v \<leftarrow> f; h v x xs odE) x)"
+   = (case_list (doE v \<leftarrow> f; g v odE) (\<lambda>x xs. doE v \<leftarrow> f; h v x xs odE) x)"
   by (simp split: list.split)
 
 lemma whenE_liftE:
@@ -216,7 +212,7 @@ lemma maybe_fail_bind_fail:
 
 lemma select_singleton[simp]:
   "select {x} = return x"
-  by (fastforce simp add: fun_eq_iff select_def return_def)
+  by (simp add: select_def return_def)
 
 lemma return_modify:
   "return () = modify id"
@@ -234,10 +230,9 @@ lemma modify_id_return:
  "modify id = return ()"
   by (simp add: simpler_modify_def return_def)
 
-
 lemma liftE_bind_return_bindE_returnOk:
   "liftE (v >>= (\<lambda>rv. return (f rv)))
-     = (liftE v >>=E (\<lambda>rv. returnOk (f rv)))"
+   = (liftE v >>=E (\<lambda>rv. returnOk (f rv)))"
   by (simp add: liftE_bindE, simp add: liftE_def returnOk_def)
 
 lemma bind_eqI:
@@ -245,12 +240,12 @@ lemma bind_eqI:
 
 lemma unlessE_throwError_returnOk:
   "(if P then returnOk v else throwError x)
-    = (unlessE P (throwError x) >>=E (\<lambda>_. returnOk v))"
+   = (unlessE P (throwError x) >>=E (\<lambda>_. returnOk v))"
   by (cases P, simp_all add: unlessE_def)
 
 lemma gets_the_bind_eq:
   "\<lbrakk> f s = Some x; g x s = h s \<rbrakk>
-    \<Longrightarrow> (gets_the f >>= g) s = h s"
+   \<Longrightarrow> (gets_the f >>= g) s = h s"
   by (simp add: gets_the_def bind_assoc exec_gets assert_opt_def)
 
 lemma zipWithM_x_modify:
@@ -265,7 +260,7 @@ lemma zipWithM_x_modify:
 
 lemma assert2:
   "(do v1 \<leftarrow> assert P; v2 \<leftarrow> assert Q; c od)
-     = (do v \<leftarrow> assert (P \<and> Q); c od)"
+   = (do v \<leftarrow> assert (P \<and> Q); c od)"
   by (simp add: assert_def split: if_split)
 
 lemma assert_opt_def2:
@@ -274,20 +269,20 @@ lemma assert_opt_def2:
 
 lemma gets_assert:
   "(do v1 \<leftarrow> assert v; v2 \<leftarrow> gets f; c v1 v2 od)
-     = (do v2 \<leftarrow> gets f; v1 \<leftarrow> assert v; c v1 v2 od)"
+   = (do v2 \<leftarrow> gets f; v1 \<leftarrow> assert v; c v1 v2 od)"
   by (simp add: simpler_gets_def return_def assert_def fail_def bind_def
          split: if_split)
 
 lemma modify_assert:
   "(do v2 \<leftarrow> modify f; v1 \<leftarrow> assert v; c v1 od)
-    = (do v1 \<leftarrow> assert v; v2 \<leftarrow> modify f; c v1 od)"
+   = (do v1 \<leftarrow> assert v; v2 \<leftarrow> modify f; c v1 od)"
   by (simp add: simpler_modify_def return_def assert_def fail_def bind_def
          split: if_split)
 
 lemma gets_fold_into_modify:
   "do x \<leftarrow> gets f; modify (g x) od = modify (\<lambda>s. g (f s) s)"
   "do x \<leftarrow> gets f; _ \<leftarrow> modify (g x); h od
-     = do modify (\<lambda>s. g (f s) s); h od"
+   = do modify (\<lambda>s. g (f s) s); h od"
   by (simp_all add: fun_eq_iff modify_def bind_assoc exec_gets
                     exec_get exec_put)
 
@@ -332,7 +327,7 @@ lemma catch_is_if:
    od"
   apply (simp add: bindE_def catch_def bind_assoc cong: if_cong)
   apply (rule bind_cong, rule refl)
-  apply (clarsimp simp: Nondet_Monad.lift_def throwError_def split: sum.splits)
+  apply (clarsimp simp: lift_def throwError_def split: sum.splits)
   done
 
 lemma liftE_K_bind: "liftE ((K_bind (\<lambda>s. A s)) x) = K_bind (liftE (\<lambda>s. A s)) x"
@@ -354,35 +349,23 @@ lemma if_to_top_of_bindE:
   "(bindE (If P x y) z) = If P (bindE x z) (bindE y z)"
   by (simp split: if_split)
 
-lemma modify_id:
-  "modify id = return ()"
-  by (simp add: modify_def get_def bind_def put_def return_def)
-
 lemma modify_modify:
   "(do x \<leftarrow> modify f; modify (g x) od) = modify (g () o f)"
   by (simp add: bind_def simpler_modify_def)
 
-lemmas modify_modify_bind = arg_cong2[where f=bind,
-  OF modify_modify refl, simplified bind_assoc]
-
-lemma select_single:
-  "select {x} = return x"
-  by (simp add: select_def return_def)
+lemmas modify_modify_bind =
+  arg_cong2[where f=bind, OF modify_modify refl, simplified bind_assoc]
 
 lemma put_then_get[unfolded K_bind_def]:
   "do put s; get od = do put s; return s od"
   by (simp add: put_def bind_def get_def return_def)
 
-lemmas put_then_get_then
-    = put_then_get[THEN bind_then_eq, simplified bind_assoc return_bind]
+lemmas put_then_get_then =
+    put_then_get[THEN bind_then_eq, simplified bind_assoc return_bind]
 
 lemma select_empty_bind[simp]:
   "select {} >>= f = select {}"
   by (simp add: select_def bind_def)
-
-lemma fail_bind[simp]:
-  "fail >>= f = fail"
-  by (simp add: bind_def fail_def)
 
 
 subsection \<open>Alternative env_steps with repeat\<close>
